project/Util.v
@@ -1,5 +1,5 @@
-Require Export Coq.Strings.String.
-Require Export Coq.Bool.Bool.
+Require Import Coq.Strings.String.
+Require Import Coq.Bool.Bool.
 
 Definition string_beq x y := if string_dec x y then true else false.
 
@@ -30,4 +30,12 @@ Qed.
 Lemma string_beq_false : forall s s', s <> s' -> string_beq s s' = false.
 Proof.
   apply string_beq_false_iff.
+Qed.
+
+(** This is useful to more easily convert 'string_beq x y = true' into x = y. *)
+Lemma string_beqP : forall x y, reflect (x = y) (string_beq x y).
+Proof.
+  intros. destruct (string_beq x y) eqn:res.
+  - apply ReflectT. apply string_beq_true_iff. assumption.
+  - apply ReflectF. apply string_beq_false_iff. assumption.
 Qed.
